proofs/refinement/PrismRefine/XPir.lean
@@ -38,8 +38,8 @@ def xStmts (P : PFunc) (ω : Nat → Nat) : Store → World → List PStmt → X
   | σ, t, .check a _ _ :: r => if truthN (a.get σ) then .fail else xStmts P ω σ t r
   | σ, t, .assume a :: r => if truthN (a.get σ) then xStmts P ω σ t r else .blocked
   | σ, t, .alloc d size kind init align :: r =>
-    xStmts P ω (σ.set d ((t.mem.alloc (size.get σ % 2 ^ 64) kind align init).2 % 2 ^ P.wd d))
-      { t with mem := (t.mem.alloc (size.get σ % 2 ^ 64) kind align init).1 } r
+    xStmts P ω (σ.set d ((t.allocW ω (size.get σ % 2 ^ 64) kind align init).2 % 2 ^ P.wd d))
+      (t.allocW ω (size.get σ % 2 ^ 64) kind align init).1 r
   | σ, t, .load d u p :: r =>
     xStmts P ω ((σ.set d (bytesVal ((loadCells t.mem (p.get σ) (P.wd d)).map (·.getD 0)) % 2 ^ P.wd d)).set u
       ((if (loadCells t.mem (p.get σ) (P.wd d)).any (·.isNone) then 1 else 0) % 2 ^ P.wd u)) t r
